Wavelet/Compile/Fn/Simulation/Invariants.lean
@@ -8,21 +8,51 @@ namespace Wavelet.Compile.Fn
 
 open Semantics Seq Dataflow Compile
 
+/-! Ghost state used for simulation that keeps track of
+the defined variables and path conditions on the `Seq` side. -/
+structure GhostState χ where
+  definedVars : List χ
+  pathConds : List (Bool × ChanName χ)
+
+@[simp, grind]
+def GhostState.empty : GhostState χ := ⟨[], []⟩
+
+@[simp, grind]
+def GhostState.init (params : List χ) : GhostState χ := ⟨params, []⟩
+
+@[simp, grind]
+def GhostState.useThenDefine [DecidableEq χ]
+  (gs : GhostState χ)
+  (usedVars : List χ)
+  (newVars : List χ) : GhostState χ :=
+  ⟨gs.definedVars.removeAll usedVars ++ newVars, gs.pathConds⟩
+
+@[simp, grind]
+def GhostState.useThenBranch [DecidableEq χ]
+  (gs : GhostState χ)
+  (condVar : χ)
+  (condVal : Bool) : GhostState χ :=
+  ⟨
+    gs.definedVars.removeAll [condVar],
+    (condVal, .var condVar gs.pathConds) :: gs.pathConds,
+  ⟩
+
 def varsToChans
   [Arity Op] [DecidableEq χ] [InterpConsts V]
+  (gs : GhostState χ)
   (ec : Seq.Config Op χ V m n) : ChanMap (ChanName χ) V :=
   λ name =>
     match name with
     | .var v pathConds =>
-      if pathConds = ec.pathConds then
+      if pathConds = gs.pathConds then
         if let some val := ec.vars.getVar v then
           [val]
         else []
       else []
     | .merge_cond v =>
-      if (true, v) ∈ ec.pathConds then
+      if (true, v) ∈ gs.pathConds then
         [InterpConsts.fromBool true]
-      else if (false, v) ∈ ec.pathConds then
+      else if (false, v) ∈ gs.pathConds then
         [InterpConsts.fromBool false]
       else []
     | .final_dest _ => []
@@ -51,7 +81,8 @@ def HasCompiledProcs
   [Arity Op] [DecidableEq χ] [InterpConsts V]
   (hnz : m > 0 ∧ n > 0)
   (ec : Seq.Config Op χ V m n)
-  (pc : Dataflow.Config Op (ChanName χ) V m n) : Prop :=
+  (pc : Dataflow.Config Op (ChanName χ) V m n)
+  (gs : GhostState χ) : Prop :=
   ∃ (rest : AtomicProcs Op (ChanName χ) V)
     (carryInLoop : Bool)
     (ctxLeft ctxCurrent ctxRight : AtomicProcs Op (ChanName χ) V),
@@ -61,31 +92,32 @@ def HasCompiledProcs
     (ec.cont = .init → ¬ carryInLoop ∧
       ctxCurrent = [] ∧
       ctxRight = [] ∧
-      ec.definedVars = [] ∧
-      ec.pathConds = []) ∧
+      gs.definedVars = [] ∧
+      gs.pathConds = []) ∧
     (∀ expr, ec.cont = .expr expr → carryInLoop ∧
-      expr.WellFormed ec.definedVars ∧
-      compileExpr hnz ec.definedVars ec.pathConds expr = ctxCurrent)
+      expr.WellFormed gs.definedVars ∧
+      compileExpr hnz gs.definedVars gs.pathConds expr = ctxCurrent)
 
 @[grind]
 def SimRel
   [Arity Op] [DecidableEq χ] [InterpConsts V]
   (hnz : m > 0 ∧ n > 0)
+  (gs : GhostState χ)
   (ec : Seq.Config Op χ V m n)
   (pc : Dataflow.Config Op (ChanName χ) V m n) : Prop :=
   -- Some invariants about the correspondence between variables and channels
-  pc.chans = varsToChans ec ∧
-  ec.definedVars.Nodup ∧
-  (∀ var, var ∈ ec.definedVars ↔ ∃ val, ec.vars.getVar var = some val) ∧
-  OrderedPathConds ec.pathConds ∧
+  pc.chans = varsToChans gs ec ∧
+  gs.definedVars.Nodup ∧
+  (∀ var, var ∈ gs.definedVars ↔ ∃ val, ec.vars.getVar var = some val) ∧
+  OrderedPathConds gs.pathConds ∧
   -- No path condition are pushed twice
-  (ec.pathConds.map Prod.snd).Nodup ∧
+  (gs.pathConds.map Prod.snd).Nodup ∧
   -- Some invariants about the "shape" of the processes
-  HasMerges m n pc.proc.atoms ec.pathConds ∧
+  HasMerges m n pc.proc.atoms gs.pathConds ∧
   ec.fn.WellFormed ∧
   pc.proc.inputs = ec.fn.params.map .input ∧
   pc.proc.outputs = (Vector.range n).map .final_dest ∧
-  HasCompiledProcs hnz ec pc
+  HasCompiledProcs hnz ec pc gs
 
 /-! Utility functions to extract facts from the simulation relation. -/
 section Utilities
@@ -94,43 +126,44 @@ variable {Op χ V S : Type*}
 variable [Arity Op] [DecidableEq χ] [InterpConsts V]
 variable {ec : Seq.Config Op χ V m n}
 variable {pc : Dataflow.Config Op (ChanName χ) V m n}
+variable {gs : GhostState χ}
 variable {hnz : m > 0 ∧ n > 0}
-variable (hsim : SimRel hnz ec pc)
+variable (hsim : SimRel hnz gs ec pc)
 
-def SimRel.vars_to_chans : pc.chans = varsToChans ec := hsim.1
+def SimRel.vars_to_chans : pc.chans = varsToChans gs ec := hsim.1
 
 def SimRel.wf_fn : ec.fn.WellFormed := by
   have ⟨_, _, _, _, _, _, h, _⟩ := hsim
   exact h
 
-def SimRel.defined_vars_nodup : ec.definedVars.Nodup := hsim.2.1
+def SimRel.defined_vars_nodup : gs.definedVars.Nodup := hsim.2.1
 
 def SimRel.defined_vars_to_get_var :
-  var ∈ ec.definedVars → ∃ val, ec.vars.getVar var = some val := by
+  var ∈ gs.definedVars → ∃ val, ec.vars.getVar var = some val := by
   have ⟨_, _, h, _⟩ := hsim
   apply (h var).mp
 
 def SimRel.get_var_to_defined_vars :
-  (∃ val, ec.vars.getVar var = some val) → var ∈ ec.definedVars := by
+  (∃ val, ec.vars.getVar var = some val) → var ∈ gs.definedVars := by
   have ⟨_, _, h, _⟩ := hsim
   apply (h var).mpr
 
 def SimRel.defined_vars_iff_get_var
-  : var ∈ ec.definedVars ↔ ∃ val, ec.vars.getVar var = some val := by
+  : var ∈ gs.definedVars ↔ ∃ val, ec.vars.getVar var = some val := by
   have ⟨_, _, h, _⟩ := hsim
   exact h var
 
-def SimRel.path_conds_nodup : (ec.pathConds.map Prod.snd).Nodup := by
+def SimRel.path_conds_nodup : (gs.pathConds.map Prod.snd).Nodup := by
   have ⟨_, _, _, _, h, _⟩ := hsim
   exact h
 
-def SimRel.path_conds_acyclic : (b, .var v ec.pathConds) ∉ ec.pathConds := by
+def SimRel.path_conds_acyclic : (b, .var v gs.pathConds) ∉ gs.pathConds := by
   intros h'
   have ⟨_, _, _, h, _⟩ := hsim
   have := h _ _ _ h'
   simp at this
 
-def SimRel.has_merges : HasMerges m n pc.proc.atoms ec.pathConds := by
+def SimRel.has_merges : HasMerges m n pc.proc.atoms gs.pathConds := by
   have ⟨_, _, _, _, _, h, _⟩ := hsim
   exact h
 
@@ -142,18 +175,18 @@ def SimRel.outputs : pc.proc.outputs = (Vector.range n).map .final_dest := by
   have ⟨_, _, _, _, _, _, _, _, h, _⟩ := hsim
   exact h
 
-def SimRel.has_compiled_procs : HasCompiledProcs hnz ec pc := by
+def SimRel.has_compiled_procs : HasCompiledProcs hnz ec pc gs := by
   have ⟨_, _, _, _, _, _, _, _, _, h⟩ := hsim
   exact h
 
 def SimRel.final_config_empty_defined_vars
-  (h : ec.cont = .init) : ec.definedVars = [] := by
+  (h : ec.cont = .init) : gs.definedVars = [] := by
   have ⟨_, _, _, _, _, _, _, _, hret, _⟩ := hsim.has_compiled_procs
   have ⟨_, _, _, h, _⟩ := hret h
   exact h
 
 def SimRel.final_config_empty_path_conds
-  (h : ec.cont = .init) : ec.pathConds = [] := by
+  (h : ec.cont = .init) : gs.pathConds = [] := by
   have ⟨_, _, _, _, _, _, _, _, hret, _⟩ := hsim.has_compiled_procs
   have ⟨_, _, _, _, h⟩ := hret h
   exact h
